\section{Pastebin (remove before handing in lol)}



\subsection{Copied source for system description equations}
\begin{subequations}
\label{eq:model_al}
\begin{align}
	\ddot{e} + K_{3} K_{ed} \dot{e} + K_{3} K_{ep} e &= K_{3} K_{ep} e_{c} \label{eq:model_se_al_elev} \\
	\ddot{p} + K_{1} K_{pd} \dot{p} + K_{1} K_{pp} p &= K_{1} K_{pp} p_{c} \label{eq:model_se_al_pitch} \\
	\dot{\lambda} &= r \label{eq:model_se_al_lambda} \\
	\dot{r} &= -K_{2} p \label{eq:model_se_al_r} 
\end{align}
\end{subequations}



\subsection{10.2.1}

\begin{subequations}
\begin{align}
	\V{x} 	&= \begin{bmatrix}\lambda & r & p & \dot{p} \end{bmatrix}\transpose \\
	u 		&= p_{c}
\end{align}
\end{subequations}

\begin{subequations}
\begin{align}
	\ddot{p} 		&= K_{1} K_{pp} (p_{c} - p) - K_{1} K_{pd} \dot{p} \\
	\dot{r} 		&= - K_{a} p \\
	\dot{\lambda} 	&= r \\
	\dot{p} 		&= \dot{p}
\end{align}
\end{subequations}

\begin{subequations}
\begin{align}
	K_{1} &= \frac{K_{f} l_{n}}{J_{p}} \\
	K_{2} &= \frac{K_{p} l_{a}}{J_{t}}
\end{align}
\end{subequations}

\begin{equation}
	\V{\dot{x}} = \M{A}_{c} \V{x} + \M{B}_{u} u \\
\end{equation}

\begin{equation}
	\V{\dot{x}} =
	\begin{bmatrix}
		0 & 1 & 0 				& 0 \\
		0 & 0 & -K_{2} 			& 0 \\
		0 & 0 & 0 				& 1 \\
		0 & 0 & -K_{1}K_{pp}	& -K_{1}K_{pd}
	\end{bmatrix}
	\V{x} +
	\begin{bmatrix}
		0 \\ 0 \\ 0 \\ K_{1}K_{pp}
	\end{bmatrix}
	p_{c}
\end{equation}



\subsection{10.2.2}

% \begin{equation}
% 	y_{k+1} = y_{k} + h f(x_{k1} y_{k})
% \end{equation}

\begin{subequations}
\begin{align}
	\V{x}_{k+1} &= \V{x}_{k} + \left( \M{A}_{c} \V{x}_{k} + \M{B}_c u_{k} \right) h \\
				&= \V{x}_{k} + h\M{A}_{c}\V{x}_{k} + h\M{B}_{c}u_{k} \\
				&= \left( \Mc{I} + h\M{A}_{c} \right) \V{x}_{k} + h\M{B}_{c}u_{k} \\
				&= \M{A}\V{x}_{k} + \M{B}u_{k}
\end{align}
\end{subequations}

\begin{subequations}
\begin{equation}
	\M{A} = \Mc{I} + h\M{A}_{c} =
	\begin{bmatrix}
		1 & h & 0 & 0 \\
		0 & 1 & -K_{2}h & 0 \\
		0 & 0 & 1 & h \\
		0 & 0 & -K_{1}K_{pp}h	& 1-K_{1}K_{pd}h
	\end{bmatrix}
\end{equation}
\begin{equation}
	\M{B} = h\M{B}_c =
	\begin{bmatrix} 0 \\ 0 \\ 0 \\ K_{1}K_{pp}h \end{bmatrix}
\end{equation}
\end{subequations}



\subsection{10.4.1}

\begin{equation}
	\V{\dot{x}}	= \M{A} \V{x} + \M{B} \V{u}
\end{equation}

\begin{equation}
	\V{x} =
	\begin{bmatrix}
		\lambda & r & p & \dot{p} & e & \dot{e}
	\end{bmatrix}\transpose
	,\qquad
	\V{u} =
	\begin{bmatrix}
		p_{c} & e_{c}
	\end{bmatrix}\transpose
\end{equation}

\begin{subequations}
\begin{align}
	\dot{\lambda}	&= r \\
	\dot{r} 		&= - K_{2} p \\
	\dot{p}			&= \dot{p} \\
	\ddot{p}		&= K_{1} K_{pp} (p_{c} - p) - K_{1} K_{pd} \dot{p} \\
	\dot{e}			&= \dot{e} \\
	\ddot{e}		&= K_{3} K_{ep} (e_{c} - e) - K_{3} K_{ed} \dot{e}
\end{align}
\end{subequations}

\begin{equation}
	\V{\dot{x}} =
	\underbrace{
		\begin{bmatrix}
			0 & 1 & 0				& 0				& 0				& 0				\\
			0 & 0 & -K_{2}			& 0				& 0				& 0				\\
			0 & 0 & 0				& 1				& 0				& 0				\\
			0 & 0 & -K_{1} K_{pp}	& -K_{1} K_{pd}	& 0				& 0				\\
			0 & 0 & 0				& 0 			& 0				& 1				\\
			0 & 0 & 0				& 0				& -K_{3} K_{ep}	& -K_{3} K_{ed} \\
		\end{bmatrix}
	}_{\M{A}_{c}}
	\V{x} +
	\underbrace{
		\begin{bmatrix}
			0				& 0				\\
			0				& 0				\\
			0				& 0				\\
			K_{1} K_{pp}	& 0				\\
			0				& 0				\\
			0				& K_{3} K_{ep}	\\
		\end{bmatrix}
	}_{\M{B}_{c}}
	\V{u}
\end{equation}



\subsection{10.4.2}

\begin{subequations}
\begin{align}
	\V{x}_{k+1}	&= \V{x}_{k} + \left( \M{A}_{c} \V{x}_{k} + \M{B}_{c} \V{u}_{k} \right) h \\
				&= \underbrace{\left( \Mc{I} + h \M{A}_{c} \right)}_{\M{A}} \V{x}_{k}
				+ \underbrace{h \M{B}_{c}}_{\M{B}} \V{u}_{k} \\
\end{align}
\end{subequations}
